Update Memory, Memory_Sems for immutable buffers, and add a writeable field in b8

vale/code/arch/x64/X64.BufferViewStore.fsti
@@ -2,7 +2,7 @@ module X64.BufferViewStore
 
 open Views
 open Interop
-module B = LowStar.Buffer
+module MB = LowStar.Monotonic.Buffer
 module BV = LowStar.BufferView
 module HS = FStar.HyperStack
 open BufferViewHelpers
@@ -13,37 +13,37 @@ module ME = X64.Memory
 module IB = Interop.Base
 
 val bv_upd_update_heap64:
-  (b:IB.b8{B.length b % 8 == 0}) ->
+  (b:IB.b8{MB.length b.IB.b % 8 == 0}) ->
   (heap:heap) ->
-  (i:nat{i < B.length b / 8}) ->
+  (i:nat{i < MB.length b.IB.b / 8}) ->
   (v:nat64) ->
-  (mem:IB.mem{B.live (IB.hs_of_mem mem) b}) ->
+  (mem:IB.mem{MB.live (IB.hs_of_mem mem) b.IB.b}) ->
    Lemma
      (requires IB.correct_down_p mem heap b)
      (ensures 
-       (let bv = BV.mk_buffer_view b view64 in
+       (let bv = BV.mk_buffer_view b.IB.b view64 in
         let addrs = IB.addrs_of_mem mem in
         let h = IB.hs_of_mem mem in
-        BV.as_buffer_mk_buffer_view b view64;
-        BV.get_view_mk_buffer_view b view64;
+        BV.as_buffer_mk_buffer_view b.IB.b view64;
+        BV.get_view_mk_buffer_view b.IB.b view64;
         BV.length_eq bv;
         let heap' = update_heap64 (addrs b + 8 `op_Multiply` i) v heap in
-        BV.upd h bv i (UInt64.uint_to_t v) == B.g_upd_seq b (get_seq_heap heap' addrs b) h))
+        BV.upd h bv i (UInt64.uint_to_t v) == MB.g_upd_seq b.IB.b (get_seq_heap heap' addrs b) h))
 
 val bv_upd_update_heap128:
-  (b:IB.b8{B.length b % 16 == 0}) ->
+  (b:IB.b8{MB.length b.IB.b % 16 == 0}) ->
   (heap:heap) ->
-  (i:nat{i < B.length b / 16}) ->
+  (i:nat{i < MB.length b.IB.b / 16}) ->
   (v:quad32) ->
-  (mem:IB.mem{B.live (IB.hs_of_mem mem) b}) ->
+  (mem:IB.mem{MB.live (IB.hs_of_mem mem) b.IB.b}) ->
    Lemma 
      (requires IB.correct_down_p mem heap b)
      (ensures (
-       let bv = BV.mk_buffer_view b view128 in
+       let bv = BV.mk_buffer_view b.IB.b view128 in
        let addrs = IB.addrs_of_mem mem in
        let h = IB.hs_of_mem mem in
-       BV.as_buffer_mk_buffer_view b view128;
-       BV.get_view_mk_buffer_view b view128;
+       BV.as_buffer_mk_buffer_view b.IB.b view128;
+       BV.get_view_mk_buffer_view b.IB.b view128;
        BV.length_eq bv;
        let heap' = update_heap128 (addrs b + 16 `op_Multiply` i) v heap in
-       BV.upd h bv i v == B.g_upd_seq b (get_seq_heap heap' addrs b) h))
+       BV.upd h bv i v == MB.g_upd_seq b.IB.b (get_seq_heap heap' addrs b) h))
