vale/code/arch/x64/X64.Memory_Sems.fst
@@ -6,7 +6,7 @@ open X64.Memory
 open Words_s
 module I = Interop
 module S = X64.Bytes_Semantics_s
-module B = LowStar.Buffer
+module MB = LowStar.Monotonic.Buffer
 module BV = LowStar.BufferView
 
 friend X64.Memory
@@ -23,6 +23,264 @@ let get_hs_heap h = I.down_up_identity h
 
 let get_heap_hs m h = I.up_down_identity h m
 
+
+val heap_shift (m1 m2:S.heap) (base:int) (n:nat) : Lemma
+  (requires (forall i. 0 <= i /\ i < n ==> m1.[base + i] == m2.[base + i]))
+  (ensures (forall i. {:pattern (m1.[i])} base <= i /\ i < base + n ==> m1.[i] == m2.[i]))
+
+let heap_shift m1 m2 base n =
+  assert (forall i. base <= i /\ i < base + n ==>
+    m1.[base + (i - base)] == m2.[base + (i - base)])
+
+open FStar.Mul
+
+val same_mem_eq_slices64 (b:buffer64{buffer_writeable b})
+                       (i:nat{i < buffer_length b})
+                       (v:nat64)
+                       (k:nat{k < buffer_length b})
+                       (h1:mem{List.memP b (IB.ptrs_of_mem h1)})
+                       (h2:mem{h2 == buffer_write b i v h1})
+                       (mem1:S.heap{IB.correct_down_p h1 mem1 b})
+                       (mem2:S.heap{IB.correct_down_p h2 mem2 b}) : Lemma
+  (requires (Seq.index (buffer_as_seq h1 b) k == Seq.index (buffer_as_seq h2 b) k))
+  (ensures (
+    k * 8 + 8 <= MB.length b.b /\
+    Seq.slice (MB.as_seq (IB.hs_of_mem h1) b.b) (k * 8) (k * 8 + 8) ==
+    Seq.slice (MB.as_seq (IB.hs_of_mem h2) b.b) (k * 8) (k * 8 + 8)))
+
+let same_mem_eq_slices64 b i v k h1 h2 mem1 mem2 =
+    let t = TUInt64 in
+    BV.as_seq_sel (IB.hs_of_mem h1) (BV.mk_buffer_view b.b (uint_view t)) k;
+    BV.as_seq_sel (IB.hs_of_mem h2) (BV.mk_buffer_view b.b (uint_view t)) k;
+    BV.put_sel (IB.hs_of_mem h1) (BV.mk_buffer_view b.b (uint_view t)) k;
+    BV.put_sel (IB.hs_of_mem h2) (BV.mk_buffer_view b.b (uint_view t)) k;
+    BV.as_buffer_mk_buffer_view b.b (uint_view t);
+    BV.get_view_mk_buffer_view b.b (uint_view t);
+    BV.view_indexing (BV.mk_buffer_view b.b (uint_view t)) k;
+    BV.length_eq (BV.mk_buffer_view b.b (uint_view t))
+
+let length_up64 (b:buffer64) (h:mem) (k:nat{k < buffer_length b}) (i:nat{i < 8}) : Lemma
+  (8 * k + i <= MB.length b.b) =
+  let vb = BV.mk_buffer_view b.b uint64_view in
+  BV.length_eq vb;
+  BV.as_buffer_mk_buffer_view b.b uint64_view;
+  BV.get_view_mk_buffer_view b.b uint64_view
+
+val same_mem_get_heap_val64 (b:buffer64{buffer_writeable b})
+                          (i:nat{i < buffer_length b})
+                          (v:nat64)
+                          (k:nat{k < buffer_length b})
+                          (h1:mem{List.memP b (IB.ptrs_of_mem h1)})
+                          (h2:mem{h2 == buffer_write b i v h1})
+                          (mem1:S.heap{IB.correct_down_p h1 mem1 b})
+                          (mem2:S.heap{IB.correct_down_p h2 mem2 b}) : Lemma
+  (requires (Seq.index (buffer_as_seq h1 b) k == Seq.index (buffer_as_seq h2 b) k))
+  (ensures (let ptr = buffer_addr b h1 + 8 * k in
+    forall i. {:pattern (mem1.[ptr+i])} i >= 0 /\ i < 8 ==> mem1.[ptr+i] == mem2.[ptr+i]))
+
+let same_mem_get_heap_val64 b j v k h1 h2 mem1 mem2 =
+  let ptr = buffer_addr b h1 + 8 * k in
+  let addr = buffer_addr b h1 in
+  let aux (i:nat{i < 8}) : Lemma (mem1.[addr+(8 * k + i)] == mem2.[addr+(8 * k +i)]) =
+    BV.as_seq_sel (IB.hs_of_mem h1) (BV.mk_buffer_view b.b uint64_view) k;
+    BV.as_seq_sel (IB.hs_of_mem h2) (BV.mk_buffer_view b.b uint64_view) k;
+    same_mem_eq_slices64 b j v k h1 h2 mem1 mem2;
+    let s1 = (Seq.slice (MB.as_seq (IB.hs_of_mem h1) b.b) (k * 8) (k * 8 + 8)) in
+    let s2 = (Seq.slice (MB.as_seq (IB.hs_of_mem h2) b.b) (k * 8) (k * 8 + 8)) in
+    assert (Seq.index s1 i == Seq.index (MB.as_seq (IB.hs_of_mem h1) b.b) (k * 8 + i));
+    length_up64 b h1 k i;
+    assert (mem1.[addr+(8 * k + i)] == UInt8.v (Seq.index (MB.as_seq (IB.hs_of_mem h1) b.b) (k * 8 + i)));
+    assert (Seq.index s2 i == Seq.index (MB.as_seq (IB.hs_of_mem h2) b.b) (k * 8 + i));
+    length_up64 b h2 k i;
+    assert (mem2.[addr+(8 * k + i)] == UInt8.v (Seq.index (MB.as_seq (IB.hs_of_mem h2) b.b) (k * 8 + i)))
+  in
+  Classical.forall_intro aux;
+  assert (forall i. addr + (8 * k + i) == ptr + i)
+
+let rec written_buffer_down64_aux1 
+  (b:buffer64{buffer_writeable b})
+  (i:nat{i < buffer_length b}) 
+  (v:nat64)
+  (h:mem{List.memP b (IB.ptrs_of_mem h)})
+  (base:nat{base == buffer_addr b h})
+  (k:nat) (h1:mem{h1 == buffer_write b i v h})
+  (mem1:S.heap{IB.correct_down h mem1})
+  (mem2:S.heap{IB.correct_down h1 mem2 /\
+               (forall j.{:pattern (mem1.[j]) \/ (mem2.[j])}
+                 base <= j /\ j < base + k * 8 ==>
+                 mem1.[j] == mem2.[j])})
+  : Lemma
+      (ensures (forall j. {:pattern (mem1.[j]) \/ (mem1.[j])}
+                  j >= base /\ j < base + 8 * i ==>
+                  mem1.[j] == mem2.[j]))
+      (decreases %[i-k]) =
+    if k >= i then ()
+    else begin
+      let ptr = base + 8 * k in
+      same_mem_get_heap_val64 b i v k h h1 mem1 mem2;
+      heap_shift mem1 mem2 ptr 8;
+      written_buffer_down64_aux1 b i v h base (k+1) h1 mem1 mem2
+    end
+
+let rec written_buffer_down64_aux2 
+  (b:buffer64{buffer_writeable b}) 
+  (i:nat{i < buffer_length b}) 
+  (v:nat64)
+  (h:mem{List.memP b (IB.ptrs_of_mem h)})
+  (base:nat{base == buffer_addr b h})
+  (n:nat{n == buffer_length b})
+  (k:nat{k > i}) (h1:mem{h1 == buffer_write b i v h})
+  (mem1:S.heap{IB.correct_down h mem1})
+  (mem2:S.heap{IB.correct_down h1 mem2 /\
+               (forall j. {:pattern (mem1.[j]) \/ (mem2.[j])}
+                 base + 8 * (i+1) <= j /\ j < base + k * 8 ==>
+                 mem1.[j] == mem2.[j])})
+  : Lemma
+      (ensures (forall j. {:pattern (mem1.[j]) \/ (mem2.[j])}
+                     j >= base + 8 * (i+1) /\ j < base + 8 * n ==>
+                     mem1.[j] == mem2.[j]))
+      (decreases %[n-k]) =
+    if k >= n then ()
+    else begin
+      let ptr = base + 8 * k in
+      same_mem_get_heap_val64 b i v k h h1 mem1 mem2;
+      heap_shift mem1 mem2 ptr 8;
+      written_buffer_down64_aux2 b i v h base n (k+1) h1 mem1 mem2
+    end
+
+let written_buffer_down64 (b:buffer64{buffer_writeable b}) (i:nat{i < buffer_length b}) (v:nat64) (h:mem)
+  : Lemma
+      (requires List.memP b (IB.ptrs_of_mem h))
+      (ensures (
+          let mem1 = I.down_mem h in
+          let h1 = buffer_write b i v h in
+          let mem2 = I.down_mem h1 in
+          let base = buffer_addr b h in
+          let n = buffer_length b in
+          forall j. {:pattern (mem1.[j]) \/ (mem2.[j])}
+               (base <= j /\ j < base + 8 * i) \/
+               (base + 8 * (i+1) <= j /\ j < base + 8 * n) ==>
+               mem1.[j] == mem2.[j]))
+  = let mem1 = I.down_mem h in
+    let h1 = buffer_write b i v h in
+    let mem2 = I.down_mem h1 in
+    let base = buffer_addr b h in
+    let n = buffer_length b in
+    written_buffer_down64_aux1 b i v h base 0 h1 mem1 mem2;
+    written_buffer_down64_aux2 b i v h base n (i+1) h1 mem1 mem2
+
+let unwritten_buffer_down (t:base_typ) (b:buffer t{buffer_writeable b})
+                          (i:nat{i < buffer_length b})
+                          (v:base_typ_as_vale_type t)
+                          (h:mem{List.memP b (IB.ptrs_of_mem h)})
+  : Lemma
+      (ensures (
+        let mem1 = I.down_mem h in
+        let h1 = buffer_write b i v h in
+        let mem2 = I.down_mem h1 in
+        forall  (a:b8{List.memP a (IB.ptrs_of_mem h) /\ a =!= b}) j. {:pattern mem1.[j]; List.memP a (IB.ptrs_of_mem h) \/ mem2.[j]; List.memP a (IB.ptrs_of_mem h)}
+          let base = (IB.addrs_of_mem h) a in
+          j >= base /\ j < base + MB.length a.b ==> mem1.[j] == mem2.[j]))
+  = let aux (a:b8{a =!= b /\ List.memP a (IB.ptrs_of_mem h)})
+      : Lemma
+        (ensures (
+          let base = (IB.addrs_of_mem h) a in
+          let mem1 = I.down_mem h in
+          let h1 = buffer_write b i v h in
+          let mem2 = I.down_mem h1 in
+          forall j.
+            j >= base /\ j < base + MB.length a.b ==>
+            mem1.[j] == mem2.[j]))
+      = if MB.length a.b = 0 then ()
+        else
+          let mem1 = I.down_mem h in
+          let h1 = buffer_write b i v h in
+          let mem2 = I.down_mem h1 in
+          let base = (IB.addrs_of_mem h) a in
+          let s0 = MB.as_seq (IB.hs_of_mem h) a.b in
+          let s1 = MB.as_seq (IB.hs_of_mem h1) a.b in
+          assert (MB.disjoint a.b b.b);
+          assert (Seq.equal s0 s1);
+          assert (forall (i:nat). {:pattern (mem1.[base + i])}
+                    i < Seq.length s0 ==> v_to_typ TUInt8 (Seq.index s0 i) == mem1.[base + i]);
+          heap_shift mem1 mem2 base (MB.length a.b)
+    in
+    Classical.forall_intro aux
+
+let store_buffer_down64_mem 
+  (b:buffer64{buffer_writeable b})
+  (i:nat{i < buffer_length b})
+  (v:nat64)
+  (h:mem{List.memP b (IB.ptrs_of_mem h)})
+  : Lemma
+      (ensures (
+        let mem1 = I.down_mem h in
+        let h1 = buffer_write b i v h in
+        let mem2 = I.down_mem h1 in
+        let base = buffer_addr b h in
+        forall (j:int). {:pattern mem1.[j] \/ mem2.[j]}
+          j < base + 8 * i \/ j >= base + 8 * (i+1) ==>
+          mem1.[j] == mem2.[j]))
+  = let mem1 = I.down_mem h in
+    let h1 = buffer_write b i v h in
+    let mem2 = I.down_mem h1 in
+    let base = buffer_addr b h in
+    let n = buffer_length b in
+    let aux (j:int)
+      : Lemma
+          (j < base + 8 * i \/ j >= base + 8 * (i+1) ==>
+           mem1.[j] == mem2.[j])
+      = if j >= base && j < base + MB.length b.b then begin
+          written_buffer_down64 b i v h;
+          length_t_eq (TUInt64) b
+        end
+        else if not (I.valid_addr h j)
+        then I.same_unspecified_down (IB.hs_of_mem h) (IB.hs_of_mem h1) (IB.ptrs_of_mem h)
+        else unwritten_buffer_down TUInt64 b i v h
+    in
+    Classical.forall_intro aux
+
+let store_buffer_aux_down64_mem (ptr:int) (v:nat64) (h:mem{writeable_mem64 ptr h})
+  : Lemma
+      (ensures (
+        let mem1 = I.down_mem h in
+        let h1 = store_mem (TUInt64) ptr v h in
+        let mem2 = I.down_mem h1 in
+        forall j. {:pattern mem1.[j] \/ mem2.[j]}
+          j < ptr \/ j >= ptr + 8 ==>
+          mem1.[j] == mem2.[j]))
+  = let t = TUInt64 in
+    let h1 = store_mem t ptr v h in
+    let b = Some?.v (find_writeable_buffer t ptr h) in
+    length_t_eq t b;
+    let i = get_addr_in_ptr t (buffer_length b) (buffer_addr b h) ptr 0 in
+    store_buffer_write t ptr v h;
+    assert (buffer_addr b h + 8 * i == ptr);
+    assert (buffer_addr b h + 8 * (i+1) == ptr + 8);
+    store_buffer_down64_mem b i v h
+
+let store_buffer_aux_down64_mem2 (ptr:int) (v:nat64) (h:mem{writeable_mem64 ptr h})
+  : Lemma
+      (ensures (
+        let h1 = store_mem (TUInt64) ptr v h in
+        let mem2 = I.down_mem h1 in
+        S.get_heap_val64 ptr mem2 == v))
+  = let t = TUInt64 in
+    let b = Some?.v (find_writeable_buffer t ptr h) in
+    length_t_eq t b;
+    let i = get_addr_in_ptr t (buffer_length b) (buffer_addr b h) ptr 0 in
+    let h1 = store_mem t ptr v h in
+    let mem2 = I.down_mem h1 in
+    store_buffer_write t ptr v h;
+    assert (Seq.index (buffer_as_seq h1 b) i == v);
+    index64_get_heap_val64 h1 b mem2 i
+
+let in_bounds64 (h:mem) (b:buffer64) (i:nat{i < buffer_length b})
+  : Lemma
+      (ensures (forall j. (IB.addrs_of_mem h) b + 8 * i <= j  /\
+                     j < (IB.addrs_of_mem h) b + 8 * i + 8 ==>
+                     j < (IB.addrs_of_mem h) b + MB.length b.b))
+  = length_t_eq (TUInt64) b
 
 let bytes_valid ptr h =
   let t = TUInt64 in
@@ -42,7 +300,7 @@ val same_mem_get_heap_val128 (b:buffer128)
                           (i:nat{i < buffer_length b})
                           (v:quad32)
                           (k:nat{k < buffer_length b})
-                          (h1:mem{List.memP b (IB.ptrs_of_mem h1)})
+                          (h1:mem{List.memP b (IB.ptrs_of_mem h1) /\ buffer_writeable b})
                           (h2:mem{h2 == buffer_write b i v h1})
                           (mem1:S.heap{IB.correct_down_p h1 mem1 b})
                           (mem2:S.heap{IB.correct_down_p h2 mem2 b}) : Lemma
@@ -54,50 +312,49 @@ val same_mem_eq_slices128 (b:buffer128)
                        (i:nat{i < buffer_length b})
                        (v:quad32)
                        (k:nat{k < buffer_length b})
-                       (h1:mem{List.memP b (IB.ptrs_of_mem h1)})
+                       (h1:mem{List.memP b (IB.ptrs_of_mem h1) /\ buffer_writeable b})
                        (h2:mem{h2 == buffer_write b i v h1})
                        (mem1:S.heap{IB.correct_down_p h1 mem1 b})
                        (mem2:S.heap{IB.correct_down_p h2 mem2 b}) : Lemma
   (requires (Seq.index (buffer_as_seq h1 b) k == Seq.index (buffer_as_seq h2 b) k))
-  (ensures (let open FStar.Mul in
-    k * 16 + 16 <= B.length b /\
-    Seq.slice (B.as_seq (IB.hs_of_mem h1) b) (k * 16) (k * 16 + 16) ==
-    Seq.slice (B.as_seq (IB.hs_of_mem h2) b) (k * 16) (k * 16 + 16)))
+  (ensures (
+    k * 16 + 16 <= MB.length b.b /\
+    Seq.slice (MB.as_seq (IB.hs_of_mem h1) b.b) (k * 16) (k * 16 + 16) ==
+    Seq.slice (MB.as_seq (IB.hs_of_mem h2) b.b) (k * 16) (k * 16 + 16)))
 
 let same_mem_eq_slices128 b i v k h1 h2 mem1 mem2 =
     let t = TUInt128 in
-    BV.as_seq_sel (IB.hs_of_mem h1) (BV.mk_buffer_view b (uint_view t)) k;
-    BV.as_seq_sel (IB.hs_of_mem h2) (BV.mk_buffer_view b (uint_view t)) k;
-    BV.put_sel (IB.hs_of_mem h1) (BV.mk_buffer_view b (uint_view t)) k;
-    BV.put_sel (IB.hs_of_mem h2) (BV.mk_buffer_view b (uint_view t)) k;
-    BV.as_buffer_mk_buffer_view b (uint_view t);
-    BV.get_view_mk_buffer_view b (uint_view t);
-    BV.view_indexing (BV.mk_buffer_view b (uint_view t)) k;
-    BV.length_eq (BV.mk_buffer_view b (uint_view t))
+    BV.as_seq_sel (IB.hs_of_mem h1) (BV.mk_buffer_view b.b (uint_view t)) k;
+    BV.as_seq_sel (IB.hs_of_mem h2) (BV.mk_buffer_view b.b (uint_view t)) k;
+    BV.put_sel (IB.hs_of_mem h1) (BV.mk_buffer_view b.b (uint_view t)) k;
+    BV.put_sel (IB.hs_of_mem h2) (BV.mk_buffer_view b.b (uint_view t)) k;
+    BV.as_buffer_mk_buffer_view b.b (uint_view t);
+    BV.get_view_mk_buffer_view b.b (uint_view t);
+    BV.view_indexing (BV.mk_buffer_view b.b (uint_view t)) k;
+    BV.length_eq (BV.mk_buffer_view b.b (uint_view t))
 
 let length_up128 (b:buffer128) (h:mem) (k:nat{k < buffer_length b}) (i:nat{i < 16}) : Lemma
-  (16 `op_Multiply` k + i <= B.length b) =
-  let vb = BV.mk_buffer_view b uint128_view in
+  (16 `op_Multiply` k + i <= MB.length b.b) =
+  let vb = BV.mk_buffer_view b.b uint128_view in
   BV.length_eq vb;
-  BV.as_buffer_mk_buffer_view b uint128_view;
-  BV.get_view_mk_buffer_view b uint128_view
+  BV.as_buffer_mk_buffer_view b.b uint128_view;
+  BV.get_view_mk_buffer_view b.b uint128_view
 
 let same_mem_get_heap_val128 b j v k h1 h2 mem1 mem2 =
   let ptr = buffer_addr b h1 + 16 `op_Multiply` k in
   let addr = buffer_addr b h1 in
   let aux (i:nat{i < 16}) : Lemma (mem1.[addr+(16 `op_Multiply` k + i)] == mem2.[addr+(16 `op_Multiply` k +i)]) =
-    BV.as_seq_sel (IB.hs_of_mem h1) (BV.mk_buffer_view b uint128_view) k;
-    BV.as_seq_sel (IB.hs_of_mem h2) (BV.mk_buffer_view b uint128_view) k;
+    BV.as_seq_sel (IB.hs_of_mem h1) (BV.mk_buffer_view b.b uint128_view) k;
+    BV.as_seq_sel (IB.hs_of_mem h2) (BV.mk_buffer_view b.b uint128_view) k;
     same_mem_eq_slices128 b j v k h1 h2 mem1 mem2;
-    let open FStar.Mul in
-    let s1 = (Seq.slice (B.as_seq (IB.hs_of_mem h1) b) (k * 16) (k * 16 + 16)) in
-    let s2 = (Seq.slice (B.as_seq (IB.hs_of_mem h2) b) (k * 16) (k * 16 + 16)) in
-    assert (Seq.index s1 i == Seq.index (B.as_seq (IB.hs_of_mem h1) b) (k * 16 + i));
+    let s1 = (Seq.slice (MB.as_seq (IB.hs_of_mem h1) b.b) (k * 16) (k * 16 + 16)) in
+    let s2 = (Seq.slice (MB.as_seq (IB.hs_of_mem h2) b.b) (k * 16) (k * 16 + 16)) in
+    assert (Seq.index s1 i == Seq.index (MB.as_seq (IB.hs_of_mem h1) b.b) (k * 16 + i));
     length_up128 b h1 k i;
-    assert (mem1.[addr+(16 * k + i)] == UInt8.v (Seq.index (B.as_seq (IB.hs_of_mem h1) b) (k * 16 + i)));
-    assert (Seq.index s2 i == Seq.index (B.as_seq (IB.hs_of_mem h2) b) (k * 16 + i));
+    assert (mem1.[addr+(16 * k + i)] == UInt8.v (Seq.index (MB.as_seq (IB.hs_of_mem h1) b.b) (k * 16 + i)));
+    assert (Seq.index s2 i == Seq.index (MB.as_seq (IB.hs_of_mem h2) b.b) (k * 16 + i));
     length_up128 b h2 k i;
-    assert (mem2.[addr+(16 * k + i)] == UInt8.v (Seq.index (B.as_seq (IB.hs_of_mem h2) b) (k * 16 + i)))
+    assert (mem2.[addr+(16 * k + i)] == UInt8.v (Seq.index (MB.as_seq (IB.hs_of_mem h2) b.b) (k * 16 + i)))
   in
   Classical.forall_intro aux;
   assert (forall i. addr + (16 `op_Multiply` k + i) == ptr + i)
@@ -105,7 +362,7 @@ let same_mem_get_heap_val128 b j v k h1 h2 mem1 mem2 =
 let in_bounds128 (h:mem) (b:buffer128) (i:nat{i < buffer_length b}) : Lemma
   (forall j. j >= h.IB.addrs b + 16 `op_Multiply` i /\ 
           j < h.IB.addrs b + 16 `op_Multiply` i + 16 ==>
-          j < h.IB.addrs b + B.length b) =
+          j < h.IB.addrs b + MB.length b.b) =
   length_t_eq TUInt128 b
 
 let bytes_valid128 ptr h =
@@ -135,7 +392,7 @@ let equiv_load_mem ptr h =
   let b = get_addr_ptr t ptr h in
   let i = get_addr_in_ptr t (buffer_length b) (buffer_addr b h) ptr 0 in
   let addr = buffer_addr b h in
-  let contents = B.as_seq h.IB.hs b in
+  let contents = MB.as_seq h.IB.hs b.b in
   let heap = get_heap h in
   index64_get_heap_val64 h b heap i;
   lemma_load_mem64 b i h
@@ -160,24 +417,23 @@ let low_lemma_store_mem64_aux
   (heap:S.heap)
   (i:nat{i < buffer_length b})
   (v:nat64)
-  (h:mem{buffer_readable h b})
+  (h:mem{buffer_readable h b /\ buffer_writeable b})
   : Lemma
     (requires IB.correct_down_p h heap b)
     (ensures (let heap' = S.update_heap64 (buffer_addr b h + 8 `op_Multiply` i) v heap in
      let h' = store_mem64 (buffer_addr b h + 8 `op_Multiply` i) v h in
-     h'.IB.hs == B.g_upd_seq b (I.get_seq_heap heap' h.IB.addrs b) h.IB.hs)) =
+     h'.IB.hs == MB.g_upd_seq b.b (I.get_seq_heap heap' h.IB.addrs b) h.IB.hs)) =
    let ptr = buffer_addr b h + 8 `op_Multiply` i in
    let heap' = S.update_heap64 ptr v heap in
    let h' = store_mem64 ptr v h in
+   lemma_store_mem64 b i v h;
    length_t_eq TUInt64 b;
-   store_buffer_write TUInt64 ptr v h;
-   let b' = get_addr_ptr TUInt64 ptr h in
-   assert (IB.disjoint_or_eq_b8 b b');
-   length_t_eq TUInt64 b';
-   bv_upd_update_heap64 b heap i v h
-
-val valid_state_store_mem64_aux: (i:int) -> (v:nat64) -> (h:mem) -> Lemma 
-  (requires valid_mem64 i h)
+   bv_upd_update_heap64 b heap i v h;
+   let bv = BV.mk_buffer_view b.IB.b Views.view64 in   
+   assert (BV.upd h.IB.hs bv i (UInt64.uint_to_t v) == h'.IB.hs)
+   
+val valid_state_store_mem64_aux: (i:nat) -> (v:nat64) -> (h:mem) -> Lemma 
+  (requires writeable_mem64 i h)
   (ensures (
     let heap = get_heap h in
     let heap' = S.update_heap64 i v heap in
@@ -204,7 +460,7 @@ let valid_state_store_mem64_aux i v h =
   Map.lemma_equal_intro mem1 mem2
   
 let low_lemma_store_mem64 b i v h =
-  lemma_valid_mem64 b i h;
+  lemma_writeable_mem64 b i h;
   lemma_store_mem64 b i v h;
   valid_state_store_mem64_aux (buffer_addr b h + 8 `op_Multiply` i) v h;
   let heap = get_heap h in
@@ -227,7 +483,7 @@ let equiv_load_mem128_aux ptr h =
   let b = get_addr_ptr t ptr h in
   let i = get_addr_in_ptr t (buffer_length b) (buffer_addr b h) ptr 0 in
   let addr = buffer_addr b h in
-  let contents = B.as_seq h.IB.hs b in
+  let contents = MB.as_seq h.IB.hs b.b in
   let heap = get_heap h in
   Opaque_s.reveal_opaque S.get_heap_val128_def;
   index128_get_heap_val128 h b heap i;
@@ -247,24 +503,23 @@ let low_lemma_store_mem128_aux
   (heap:S.heap)
   (i:nat{i < buffer_length b})
   (v:quad32)
-  (h:mem{buffer_readable h b})
+  (h:mem{buffer_readable h b /\ buffer_writeable b})
   : Lemma
     (requires IB.correct_down_p h heap b)
     (ensures (let heap' = S.update_heap128 (buffer_addr b h + 16 `op_Multiply` i) v heap in
      let h' = store_mem128 (buffer_addr b h + 16 `op_Multiply` i) v h in
-     h'.IB.hs == B.g_upd_seq b (I.get_seq_heap heap' h.IB.addrs b) h.IB.hs)) =
+     h'.IB.hs == MB.g_upd_seq b.b (I.get_seq_heap heap' h.IB.addrs b) h.IB.hs)) =
    let ptr = buffer_addr b h + 16 `op_Multiply` i in
    let heap' = S.update_heap128 ptr v heap in
    let h' = store_mem128 ptr v h in
+   lemma_store_mem128 b i v h;
    length_t_eq TUInt128 b;
-   store_buffer_write TUInt128 ptr v h;
-   let b' = get_addr_ptr TUInt128 ptr h in
-   assert (IB.disjoint_or_eq_b8 b b');
-   length_t_eq TUInt128 b';
-   bv_upd_update_heap128 b heap i v h
+   bv_upd_update_heap128 b heap i v h;
+   let bv = BV.mk_buffer_view b.IB.b Views.view128 in   
+   assert (BV.upd h.IB.hs bv i v == h'.IB.hs)
 
 val valid_state_store_mem128_aux: (i:int) -> (v:quad32) -> (h:mem) -> Lemma 
-  (requires valid_mem128 i h)
+  (requires writeable_mem128 i h)
   (ensures (
     let heap = get_heap h in
     let heap' = S.update_heap128 i v heap in
@@ -272,146 +527,18 @@ val valid_state_store_mem128_aux: (i:int) -> (v:quad32) -> (h:mem) -> Lemma
     heap' == I.down_mem h' 
   ))
 
-(*
-let rec written_buffer_down128_aux1 (b:buffer128) (i:nat{i < buffer_length b}) (v:quad32)
-      (ps:list b8{IB.list_disjoint_or_eq ps /\ List.memP b ps})
-      (h:mem{forall x. List.memP x ps ==> List.memP x (IB.ptrs_of_mem h)})
-      (base:nat{base == buffer_addr b h})
-      (k:nat) (h1:mem{h1 == buffer_write b i v h})
-      (mem1:S.heap{I.correct_down h.hs h.addrs ps mem1})
-      (mem2:S.heap{
-      (I.correct_down h1.hs h.addrs ps mem2) /\
-      (forall j. base <= j /\ j < base + k `op_Multiply` 16 ==> mem1.[j] == mem2.[j])}) :
-      Lemma (requires True)
-      (ensures (forall j. j >= base /\ j < base + 16 `op_Multiply` i ==> mem1.[j] == mem2.[j]))
-      (decreases %[i-k]) =
-    if k >= i then ()
-    else begin
-      let ptr = base + 16 `op_Multiply` k in
-      same_mem_get_heap_val128 b i v k h h1 mem1 mem2;
-      heap_shift mem1 mem2 ptr 16;
-      written_buffer_down128_aux1 b i v ps h base (k+1) h1 mem1 mem2
-    end
-
-let rec written_buffer_down128_aux2 (b:buffer128) (i:nat{i < buffer_length b}) (v:quad32)
-      (ps:list b8{I.list_disjoint_or_eq ps /\ List.memP b ps})
-      (h:mem{forall x. List.memP x ps ==> List.memP x h.ptrs})
-      (base:nat{base == buffer_addr b h})
-      (n:nat{n == buffer_length b})
-      (k:nat{k > i}) (h1:mem{h1 == buffer_write b i v h})
-      (mem1:S.heap{I.correct_down h.hs h.addrs ps mem1})
-      (mem2:S.heap{
-      (I.correct_down h1.hs h.addrs ps mem2) /\
-      (forall j. base + 16 `op_Multiply` (i+1) <= j /\ j < base + k `op_Multiply` 16 ==>
-      mem1.[j] == mem2.[j])}) :
-      Lemma
-      (requires True)
-      (ensures (forall j. j >= base + 16 `op_Multiply` (i+1) /\ j < base + 16 `op_Multiply` n ==>
-        mem1.[j] == mem2.[j]))
-      (decreases %[n-k]) =
-    if k >= n then ()
-    else begin
-      let ptr = base + 16 `op_Multiply` k in
-      same_mem_get_heap_val128 b i v k h h1 mem1 mem2;
-      heap_shift mem1 mem2 ptr 16;
-      written_buffer_down128_aux2 b i v ps h base n (k+1) h1 mem1 mem2
-    end
-
-let written_buffer_down128 (b:buffer128) (i:nat{i < buffer_length b}) (v:quad32)
-  (ps: list b8{I.list_disjoint_or_eq ps /\ List.memP b ps}) (h:mem{forall x. List.memP x ps ==> List.memP x h.ptrs}) :
-  Lemma (
-    let mem1 = I.down_mem h.hs h.addrs ps in
-    let h1 = buffer_write b i v h in
-    let mem2 = I.down_mem h1.hs h.addrs ps in
-    let base = buffer_addr b h in
-    let n = buffer_length b in
-    forall j. (base <= j /\ j < base + 16 `op_Multiply` i) \/
-         (base + 16 `op_Multiply` (i+1) <= j /\ j < base + 16 `op_Multiply` n) ==>
-         mem1.[j] == mem2.[j]) =
-    let mem1 = I.down_mem h.hs h.addrs ps in
-    let h1 = buffer_write b i v h in
-    let mem2 = I.down_mem h1.hs h.addrs ps in
-    let base = buffer_addr b h in
-    let n = buffer_length b in
-    written_buffer_down128_aux1 b i v ps h base 0 h1 mem1 mem2;
-    written_buffer_down128_aux2 b i v ps h base n (i+1) h1 mem1 mem2
-
-let store_buffer_down128_mem (b:buffer128) (i:nat{i < buffer_length b}) (v:quad32)
-  (ps: list b8{I.list_disjoint_or_eq ps /\ List.memP b ps})
-  (h:mem{forall x. List.memP x ps ==> List.memP x h.ptrs}) :
-  Lemma (
-    let mem1 = I.down_mem h.hs h.addrs ps in
-    let h1 = buffer_write b i v h in
-    let mem2 = I.down_mem h1.hs h.addrs ps in
-    let base = buffer_addr b h in
-    forall j. j < base + 16 `op_Multiply` i \/ j >= base + 16 `op_Multiply` (i+1) ==>
-      mem1.[j] == mem2.[j]) =
-    let mem1 = I.down_mem h.hs h.addrs ps in
-    let h1 = buffer_write b i v h in
-    let mem2 = I.down_mem h1.hs h.addrs ps in
-    let base = buffer_addr b h in
-    let n = buffer_length b in
-    let aux (j:int) : Lemma
-      (j < base + 16 `op_Multiply` i \/ j >= base + 16 `op_Multiply` (i+1) ==>
-      mem1.[j] == mem2.[j]) =
-        if j >= base && j < base + B.length b then begin
-          written_buffer_down128 b i v ps h;
-          length_t_eq (TBase TUInt128) b
-        end
-        else (
-        I.same_unspecified_down h.hs h1.hs h.addrs ps;
-        unwritten_buffer_down (TBase TUInt128) b i v ps h;
-        ()
-        )
-    in Classical.forall_intro aux
-
-let store_buffer_aux_down128_mem (ptr:int) (v:quad32) (h:mem{valid_mem128 ptr h}) : Lemma (
-  let mem1 = I.down_mem h in
-  let h1 = store_mem TUInt128 ptr v h in
-  let mem2 = I.down_mem h1 in
-  forall j. j < ptr \/ j >= ptr + 16 ==> mem1.[j] == mem2.[j]) =
-  let t = TUInt128 in
-  let h1 = store_mem t ptr v h in
-  let b = get_addr_ptr t ptr h in
-  length_t_eq t b;
-  let i = get_addr_in_ptr t (buffer_length b) (buffer_addr b h) ptr 0 in
-  store_buffer_write t ptr v h;
-  assert (buffer_addr b h + 16 `op_Multiply` i == ptr);
-  assert (buffer_addr b h + 16 `op_Multiply` (i+1) == ptr + 16)
-  store_buffer_down128_mem b i v h
-
-let store_buffer_aux_down128_mem2 (ptr:int) (v:quad32) (h:mem{valid_mem128 ptr h}) : Lemma (
-  let h1 = store_mem_aux (TBase TUInt128) ptr h.ptrs v h in
-  let mem2 = I.down_mem h1.hs h.addrs h.ptrs in
-  Mkfour
-    (S.get_heap_val32 ptr mem2)
-    (S.get_heap_val32 (ptr+4) mem2)
-    (S.get_heap_val32 (ptr+8) mem2)
-    (S.get_heap_val32 (ptr+12) mem2)
-  == v) =
-  let t = TBase TUInt128 in
-  let b = get_addr_ptr t ptr h h.ptrs in
-  length_t_eq t b;
-  let i = get_addr_in_ptr t (buffer_length b) (buffer_addr b h) ptr 0 in
-  let h1 = store_mem_aux t ptr h.ptrs v h in
-  let mem2 = I.down_mem h1.hs h.addrs h.ptrs in
-  store_buffer_write t ptr v h h.ptrs;
-  assert (Seq.index (buffer_as_seq h1 b) i == v);
-  index128_get_heap_val128 h1 b mem2 i;
-  ()
-*)
-
-open FStar.Mul
-
-let rec written_buffer_down128_aux1 (b:buffer128) (i:nat{i < buffer_length b}) (v:quad32)
-      (h:mem{List.memP b h.IB.ptrs})
-      (base:nat{base == buffer_addr b h})
-      (k:nat) (h1:mem{h1 == buffer_write b i v h})
-      (mem1:S.heap{IB.correct_down h mem1})
-      (mem2:S.heap{IB.correct_down h1 mem2 /\
-                   (forall j.{:pattern (mem1.[j]) \/ (mem2.[j])}
-                     base <= j /\ j < base + k * 16 ==>
-                     mem1.[j] == mem2.[j])})
+let rec written_buffer_down128_aux1 
+  (b:buffer128{buffer_writeable b})
+  (i:nat{i < buffer_length b}) 
+  (v:quad32)
+  (h:mem{List.memP b h.IB.ptrs})
+  (base:nat{base == buffer_addr b h})
+  (k:nat) (h1:mem{h1 == buffer_write b i v h})
+  (mem1:S.heap{IB.correct_down h mem1})
+  (mem2:S.heap{IB.correct_down h1 mem2 /\
+               (forall j.{:pattern (mem1.[j]) \/ (mem2.[j])}
+                 base <= j /\ j < base + k * 16 ==>
+                 mem1.[j] == mem2.[j])})
   : Lemma
       (ensures (forall j. {:pattern (mem1.[j]) \/ (mem1.[j])}
                   j >= base /\ j < base + 16 * i ==>
@@ -425,16 +552,19 @@ let rec written_buffer_down128_aux1 (b:buffer128) (i:nat{i < buffer_length b}) (
       written_buffer_down128_aux1 b i v h base (k+1) h1 mem1 mem2
     end
 
-let rec written_buffer_down128_aux2 (b:buffer128) (i:nat{i < buffer_length b}) (v:quad32)
-      (h:mem{List.memP b h.IB.ptrs})
-      (base:nat{base == buffer_addr b h})
-      (n:nat{n == buffer_length b})
-      (k:nat{k > i}) (h1:mem{h1 == buffer_write b i v h})
-      (mem1:S.heap{IB.correct_down h mem1})
-      (mem2:S.heap{IB.correct_down h1 mem2 /\
-                   (forall j. {:pattern (mem1.[j]) \/ (mem2.[j])}
-                     base + 16 * (i+1) <= j /\ j < base + k * 16 ==>
-                     mem1.[j] == mem2.[j])})
+let rec written_buffer_down128_aux2 
+  (b:buffer128{buffer_writeable b})
+  (i:nat{i < buffer_length b})
+  (v:quad32)
+  (h:mem{List.memP b h.IB.ptrs})
+  (base:nat{base == buffer_addr b h})
+  (n:nat{n == buffer_length b})
+  (k:nat{k > i}) (h1:mem{h1 == buffer_write b i v h})
+  (mem1:S.heap{IB.correct_down h mem1})
+  (mem2:S.heap{IB.correct_down h1 mem2 /\
+               (forall j. {:pattern (mem1.[j]) \/ (mem2.[j])}
+                 base + 16 * (i+1) <= j /\ j < base + k * 16 ==>
+                 mem1.[j] == mem2.[j])})
   : Lemma
       (ensures (forall j. {:pattern (mem1.[j]) \/ (mem2.[j])}
                      j >= base + 16 * (i+1) /\ j < base + 16 * n ==>
@@ -450,7 +580,7 @@ let rec written_buffer_down128_aux2 (b:buffer128) (i:nat{i < buffer_length b}) (
 
 let written_buffer_down128 (b:buffer128) (i:nat{i < buffer_length b}) (v:quad32) (h:mem)
   : Lemma
-      (requires List.memP b h.IB.ptrs)
+      (requires List.memP b h.IB.ptrs /\ buffer_writeable b)
       (ensures (
           let mem1 = I.down_mem h in
           let h1 = buffer_write b i v h in
@@ -469,8 +599,11 @@ let written_buffer_down128 (b:buffer128) (i:nat{i < buffer_length b}) (v:quad32)
     written_buffer_down128_aux1 b i v h base 0 h1 mem1 mem2;
     written_buffer_down128_aux2 b i v h base n (i+1) h1 mem1 mem2
 
-let store_buffer_down128_mem (b:buffer128) (i:nat{i < buffer_length b}) (v:quad32)
-                            (h:mem{List.memP b h.IB.ptrs})
+let store_buffer_down128_mem 
+  (b:buffer128{buffer_writeable b})
+  (i:nat{i < buffer_length b})
+  (v:quad32)
+  (h:mem{List.memP b h.IB.ptrs})
   : Lemma
       (ensures (
         let mem1 = I.down_mem h in
@@ -489,7 +622,7 @@ let store_buffer_down128_mem (b:buffer128) (i:nat{i < buffer_length b}) (v:quad3
       : Lemma
           (j < base + 16 * i \/ j >= base + 16 * (i+1) ==>
            mem1.[j] == mem2.[j])
-      = if j >= base && j < base + B.length b then begin
+      = if j >= base && j < base + MB.length b.b then begin
           written_buffer_down128 b i v h;
           length_t_eq TUInt128 b
         end
@@ -499,7 +632,7 @@ let store_buffer_down128_mem (b:buffer128) (i:nat{i < buffer_length b}) (v:quad3
     in
     Classical.forall_intro aux
 
-let store_buffer_aux_down128_mem (ptr:int) (v:quad32) (h:mem{valid_mem128 ptr h})
+let store_buffer_aux_down128_mem (ptr:int) (v:quad32) (h:mem{writeable_mem128 ptr h})
   : Lemma
       (ensures (
         let mem1 = I.down_mem h in
@@ -510,7 +643,7 @@ let store_buffer_aux_down128_mem (ptr:int) (v:quad32) (h:mem{valid_mem128 ptr h}
           mem1.[j] == mem2.[j]))
   = let t = TUInt128 in
     let h1 = store_mem t ptr v h in
-    let b = get_addr_ptr t ptr h in
+    let b = Some?.v (find_writeable_buffer t ptr h) in
     length_t_eq t b;
     let i = get_addr_in_ptr t (buffer_length b) (buffer_addr b h) ptr 0 in
     store_buffer_write t ptr v h;
@@ -518,7 +651,7 @@ let store_buffer_aux_down128_mem (ptr:int) (v:quad32) (h:mem{valid_mem128 ptr h}
     assert (buffer_addr b h + 16 * (i+1) == ptr + 16);
     store_buffer_down128_mem b i v h
 
-let store_buffer_aux_down128_mem2 (ptr:int) (v:quad32) (h:mem{valid_mem128 ptr h})
+let store_buffer_aux_down128_mem2 (ptr:int) (v:quad32) (h:mem{writeable_mem128 ptr h})
   : Lemma
       (ensures (
         let h1 = store_mem TUInt128 ptr v h in
@@ -530,7 +663,7 @@ let store_buffer_aux_down128_mem2 (ptr:int) (v:quad32) (h:mem{valid_mem128 ptr h
           (S.get_heap_val32 (ptr+12) mem2)
         == v)) =
     let t = TUInt128 in
-    let b = get_addr_ptr t ptr h in
+    let b = Some?.v (find_writeable_buffer t ptr h) in
     length_t_eq t b;
     let i = get_addr_in_ptr t (buffer_length b) (buffer_addr b h) ptr 0 in
     let h1 = store_mem t ptr v h in
